checker/checkTrace.mli
@@ -1,0 +1,4 @@
+(* Check correspondence between a model
+ * and the initial clauses of a resolution proof. *)
+val assumptions : Model.t -> (int, MTypes.lit) Hashtbl.t ->
+  Genlex.token Stream.t -> MTypes.clause list
